::: {style="DISPLAY: none"}
[](ms-xhelp:///?Id=d2h_url_template){#d2h_url_template}![](!package_url!){#d2h_package_url style="WIDTH: 0px; DISPLAY: none; HEIGHT: 0px"}
:::

::::: {#nsbanner .d2h_main_nsbanner style="BORDER-BOTTOM: #999999 1px solid; POSITION: relative; PADDING-BOTTOM: 0px; BACKGROUND-COLOR: transparent; PADDING-LEFT: 0px; PADDING-RIGHT: 0px; DISPLAY: none; BORDER-TOP: #999999 1px solid; PADDING-TOP: 0px; LEFT: 0px"}
:::: {#TitleRow .d2h_main_titlerow style="PADDING-BOTTOM: 4px; BACKGROUND-COLOR: transparent; PADDING-LEFT: 22px; WIDTH: 100%; PADDING-RIGHT: 10px; DISPLAY: none; PADDING-TOP: 4px"}
::: {#ienav .d2h_main_ienav style="DISPLAY: none"}
[](ms-xhelp:///?Id=dd91bec0-4ed5-41da-b70b-09ec9a34671a){#D2HPrevious .D2HPreviousEnabled}  [](ms-xhelp:///?Id=3920f78e-ccc2-4b50-b4be-311a9b9a514d){#D2HNext .D2HNextEnabled}
:::
::::
:::::

:::: {#nstext .d2h_main_nstext style="PADDING-BOTTOM: 10px; BACKGROUND-COLOR: transparent; PADDING-LEFT: 22px; PADDING-RIGHT: 10px; HEIGHT: 100%; OVERFLOW: auto; PADDING-TOP: 5px" hasuserbackground="true" valign="bottom"}
::: {#d2h_breadcrumbs .d2h_breadcrumbs}
[Essential Studio User Guide Documentation](ms-xhelp:///?Id=12457748-09e3-4d74-a240-8e049cedf030){.d2h_breadcrumbsNormal}[ \> ]{.d2h_breadcrumbsLinkSeparator}[Reporting Edition](ms-xhelp:///?Id=027aa5b6-6676-4f93-ad23-c20e8c45792e){.d2h_breadcrumbsNormal}[ \> ]{.d2h_breadcrumbsLinkSeparator}[Essential Calculate](ms-xhelp:///?Id=2ea52c7f-a332-43bd-9ca7-2ea0898ff54e){.d2h_breadcrumbsNormal}[ \> ]{.d2h_breadcrumbsLinkSeparator}[Concepts and Features](ms-xhelp:///?Id=91222e44-d3ca-4392-8f0f-41bd2ae3dd3f){.d2h_breadcrumbsNormal}[ \> ]{.d2h_breadcrumbsLinkSeparator}[Function Reference Section](ms-xhelp:///?Id=64c2cb3d-2548-4fe4-b0d1-0c2249ee26c8){.d2h_breadcrumbsNormal}
:::

### FISHERINV {#fisherinv style="tab-stops: 0pt"}

 

Returns the inverse of the Fisher transformation. If y = FISHER(x), then FISHERINV(y) = x.

 

**Syntax**

**FISHERINV(y)**

 

where:

y is the value for which you want to perform the inverse of the transformation.

 

**Remarks**

 

[·      ]{style="FONT-FAMILY: Symbol"}The equation for the inverse of the Fisher transformation is:

[]{style="FONT-FAMILY: 'Trebuchet MS','sans-serif'; COLOR: #15428b; FONT-SIZE: 9pt"} 

![](ImagesExt/image18_60.png){border="0"}

 

[]{#related-topics}
::::
